arm+arm-hyp+aarch64: SGISignalCap proofs
Signed-off-by: Gerwin Klein <gerwin.klein@proofcraft.systems>

proof/refine/ARM/Invariants_H.thy
@@ -45,6 +45,13 @@ lemma le_maxDomain_eq_less_numDomains:
         "y \<le> maxDomain \<longleftrightarrow> unat y < Kernel_Config.numDomains"
   by (auto simp: Kernel_Config.numDomains_def maxDomain_def word_le_nat_alt)
 
+context begin interpretation Arch .
+requalify_consts
+  SGISignalCap
+end
+
+definition isArchSGISignalCap :: "capability \<Rightarrow> bool" where
+  "isArchSGISignalCap cap \<equiv> \<exists>irq targets. cap = ArchObjectCap (SGISignalCap irq targets)"
 
 context begin interpretation Arch . (*FIXME: arch_split*)
 \<comment> \<open>---------------------------------------------------------------------------\<close>
@@ -326,6 +333,7 @@ where
 | "acapBits (PageCap d x y sz z) = pageBitsForSize sz"
 | "acapBits (PageTableCap x y) = 10"
 | "acapBits (PageDirectoryCap x y) = 14"
+| "acapBits (SGISignalCap _ _) = 0"
 end
 
 
@@ -439,7 +447,8 @@ where valid_cap'_def:
             0 < asid \<and> asid \<le> 2^asid_bits - 1 \<and> ref < pptrBase)
   | PageDirectoryCap ref mapdata \<Rightarrow>
     page_directory_at' ref s \<and>
-    case_option True (\<lambda>asid. 0 < asid \<and> asid \<le> 2^asid_bits - 1) mapdata))"
+    case_option True (\<lambda>asid. 0 < asid \<and> asid \<le> 2^asid_bits - 1) mapdata
+  | SGISignalCap _ _ \<Rightarrow> True))"
 
 abbreviation (input)
   valid_cap'_syn :: "kernel_state \<Rightarrow> capability \<Rightarrow> bool" ("_ \<turnstile>'' _" [60, 60] 61)
@@ -631,20 +640,23 @@ where
 
 definition
   "valid_badges m \<equiv>
-  \<forall>p p' cap node cap' node'.
-    m p = Some (CTE cap node) \<longrightarrow>
-    m p' = Some (CTE cap' node') \<longrightarrow>
-    (m \<turnstile> p \<leadsto> p') \<longrightarrow>
-    (sameRegionAs cap cap') \<longrightarrow>
-    (isEndpointCap cap \<longrightarrow>
-     capEPBadge cap \<noteq> capEPBadge cap' \<longrightarrow>
-     capEPBadge cap' \<noteq> 0 \<longrightarrow>
-     mdbFirstBadged node')
-    \<and>
-    (isNotificationCap cap \<longrightarrow>
-     capNtfnBadge cap \<noteq> capNtfnBadge cap' \<longrightarrow>
-     capNtfnBadge cap' \<noteq> 0 \<longrightarrow>
-     mdbFirstBadged node')"
+   \<forall>p p' cap node cap' node'.
+     m p = Some (CTE cap node) \<longrightarrow>
+     m p' = Some (CTE cap' node') \<longrightarrow>
+     m \<turnstile> p \<leadsto> p' \<longrightarrow>
+     (sameRegionAs cap cap' \<longrightarrow>
+      (isEndpointCap cap \<longrightarrow>
+       capEPBadge cap \<noteq> capEPBadge cap' \<longrightarrow>
+      capEPBadge cap' \<noteq> 0 \<longrightarrow>
+       mdbFirstBadged node')
+     \<and>
+      (isNotificationCap cap \<longrightarrow>
+       capNtfnBadge cap \<noteq> capNtfnBadge cap' \<longrightarrow>
+       capNtfnBadge cap' \<noteq> 0 \<longrightarrow>
+       mdbFirstBadged node'))
+     \<and>
+     (isArchSGISignalCap cap' \<longrightarrow> cap \<noteq> cap' \<longrightarrow>
+      mdbFirstBadged node')"
 
 fun (sequential)
   untypedRange :: "capability \<Rightarrow> word32 set"
@@ -660,6 +672,7 @@ where
 | "acapClass (PageCap d x y sz z)   = PhysicalClass"
 | "acapClass (PageTableCap x y)     = PhysicalClass"
 | "acapClass (PageDirectoryCap x y) = PhysicalClass"
+| "acapClass (SGISignalCap _ _ )    = IRQClass"
 
 primrec
   capClass :: "capability \<Rightarrow> capclass"
@@ -725,6 +738,7 @@ definition
   m p = Some (CTE cap n) \<longrightarrow>
   m p' = Some (CTE cap' n') \<longrightarrow>
   sameRegionAs cap cap' \<longrightarrow>
+  \<not>isArchSGISignalCap cap \<longrightarrow>
   p \<noteq> p' \<longrightarrow>
   (m \<turnstile> p \<leadsto>\<^sup>+ p' \<or> m \<turnstile> p' \<leadsto>\<^sup>+ p) \<and>
   (m \<turnstile> p \<leadsto>\<^sup>+ p' \<longrightarrow> is_chunk m cap p p') \<and>
@@ -2971,7 +2985,7 @@ lemma class_linksD:
 
 lemma mdb_chunkedD:
   "\<lbrakk> m p = Some (CTE cap n); m p' = Some (CTE cap' n');
-     sameRegionAs cap cap'; p \<noteq> p'; mdb_chunked m \<rbrakk>
+     sameRegionAs cap cap'; p \<noteq> p'; \<not>isArchSGISignalCap cap; mdb_chunked m \<rbrakk>
   \<Longrightarrow> (m \<turnstile> p \<leadsto>\<^sup>+ p' \<or> m \<turnstile> p' \<leadsto>\<^sup>+ p) \<and>
      (m \<turnstile> p \<leadsto>\<^sup>+ p' \<longrightarrow> is_chunk m cap p p') \<and>
      (m \<turnstile> p' \<leadsto>\<^sup>+ p \<longrightarrow> is_chunk m cap' p' p)"
